Define C array access and update operations
Add c_ptr_at for computing the gref of array element i at base + i *
stride. Array dereference and update use the existing locale-provided
dereference_by_value_raw_fun and update_raw_fun on the computed gref.

Signed-off-by: Dominic Mulligan <dominic.p.mulligan@gmail.com>

Shallow_Micro_C/C_Memory_Operations.thy
@@ -41,6 +41,25 @@ lemma c_ptr_add_null_guard:
   shows \<open>\<not> is_null_nat (c_ptr_add p n stride)\<close>
   using assms by (simp add: is_null_nat_def c_ptr_add_def)
 
+section \<open>Array Element References\<close>
+
+text \<open>
+  In C, @{text "p[i]"} is defined as @{text "*(p + i)"}. The function @{text c_ptr_at}
+  computes the @{type gref} for the i-th element of an array starting at @{text p}.
+  The actual dereference or update is performed by locale-provided operations
+  such as @{text dereference_by_value_raw_fun} and @{text update_raw_fun}.
+\<close>
+
+definition c_ptr_at :: \<open>(nat, 'b) gref \<Rightarrow> nat \<Rightarrow> nat \<Rightarrow> (nat, 'b) gref\<close> where
+  \<open>c_ptr_at p i stride \<equiv> c_ptr_add p i stride\<close>
+
+lemma c_ptr_at_address [simp]:
+  \<open>gref_address (c_ptr_at p i stride) = gref_address p + i * stride\<close>
+  by (simp add: c_ptr_at_def)
+
+lemma c_ptr_at_zero [simp]: \<open>c_ptr_at p 0 stride = p\<close>
+  by (simp add: c_ptr_at_def)
+
 section \<open>C Pointer Subtraction\<close>
 
 definition c_ptr_diff :: \<open>(nat, 'b) gref \<Rightarrow> (nat, 'b) gref \<Rightarrow> nat \<Rightarrow> nat\<close> where
